compiler/backend/passes/proofs/thunk_split_Delay_LamProofScript.sml
@@ -3564,11 +3564,11 @@ QED
 
 Theorem split_Delayed_Lam_soundness:
   ∀e vc e_out vc_out.
+     split_Delayed_Lam e vc (empty compare) = (e_out, vc_out) ∧
      closed (exp_of e) ∧
      boundvars (exp_of e) ⊆ set_of vc ∧
      vars_ok vc ∧
-     cexp_wf e ∧
-     split_Delayed_Lam e vc (empty compare) = (e_out, vc_out)
+     cexp_wf e
      ⇒ cexp_wf e_out ∧
        cns_arities e = cns_arities e_out ∧
        boundvars (exp_of e_out) ⊆ set_of vc_out ∧
